ProjectEulerSolutions/P8.lean
@@ -1,35 +1,6 @@
 import ProjectEulerStatements.P8
 namespace ProjectEulerSolutions.P8
 
-abbrev numberStr : String :=
-  "73167176531330624919225119674426574742355349194934" ++
-  "96983520312774506326239578318016984801869478851843" ++
-  "85861560789112949495459501737958331952853208805511" ++
-  "12540698747158523863050715693290963295227443043557" ++
-  "66896648950445244523161731856403098711121722383113" ++
-  "62229893423380308135336276614282806444486645238749" ++
-  "30358907296290491560440772390713810515859307960866" ++
-  "70172427121883998797908792274921901699720888093776" ++
-  "65727333001053367881220235421809751254540594752243" ++
-  "52584907711670556013604839586446706324415722155397" ++
-  "53697817977846174064955149290862569321978468622482" ++
-  "83972241375657056057490261407972968652414535100474" ++
-  "82166370484403199890008895243450658541227588666881" ++
-  "16427171479924442928230863465674813919123162824586" ++
-  "17866458359124566529476545682848912883142607690042" ++
-  "24219022671055626321111109370544217506941658960408" ++
-  "07198403850962455444362981230987879927244284909188" ++
-  "84580156166097919133875499200524063689912560717606" ++
-  "05886116467109405077541002256983155200055935729725" ++
-  "71636269561882670428252483600823257530420752963450"
-
-
-def digitsArray (s : String) : Array Nat :=
-  s.data.foldl (fun acc c => acc.push (c.toNat - '0'.toNat)) #[]
-
-def digitsList (s : String) : List Nat :=
-  s.data.map (fun c => c.toNat - '0'.toNat)
-
 def hasZero : List Nat -> Bool
   | [] => false
   | x :: xs => x == 0 || hasZero xs
@@ -47,17 +18,16 @@ def productLoop (k : Nat) : List Nat -> List Nat
         else
           ProjectEulerStatements.P8.listProduct window :: products
 
-def maxAdjacentProduct (num : String) (k : Nat) : Nat :=
-  let digits := digitsList num
+def maxAdjacentProduct (digits : List Nat) (k : Nat) : Nat :=
   if k == 0 then
     if digits.isEmpty then 0 else 1
   else
     ProjectEulerStatements.P8.listMax (productLoop k digits)
 
 
-def solve (n k : Nat) : Nat :=
-  maxAdjacentProduct (toString n) k
+def solve (digits : List Nat) (k : Nat) : Nat :=
+  maxAdjacentProduct digits k
 
-example : solve ProjectEulerStatements.P8.bigNumber 4 = 5832 := by
+example : solve ProjectEulerStatements.P8.digits1000 4 = 5832 := by
   native_decide
 end ProjectEulerSolutions.P8
